TouhouFormal/ECL.lean
@@ -8,6 +8,7 @@ import TouhouFormal.ECL.Instruction
 import TouhouFormal.ECL.Step
 import TouhouFormal.ECL.Operand
 import TouhouFormal.ECL.Body
+import TouhouFormal.ECL.Comparison
 import TouhouFormal.ECL.Stack
 import TouhouFormal.ECL.Arithmetic
 import TouhouFormal.ECL.Assignment
